theories/automation.v
@@ -537,6 +537,22 @@ Proof.
   by apply (IH (_, _)).
 Qed.
 
+Fixpoint regcol_lookup_field (r f : string) (regs : list (reg_kind * valu_shape)) : option (bool * valu_shape) :=
+  match regs with
+  | (r', s)::regs' =>
+      if reg_kind_eqb (KindField r f) r' then
+        Some (true, s)
+      else if reg_kind_eqb (KindReg r) r' then
+        match s with
+        | StructShape ss => (λ x, (false, x.2.2)) <$> list_find_bool (λ x, x.1 =? f)%string ss
+        | ExactShape (RegVal_Struct rs) =>
+            (λ x, (false, ExactShape x.2.2)) <$> list_find_bool (λ x, x.1 =? f)%string rs
+        | _ => None
+        end
+      else regcol_lookup_field r f regs'
+  | [] => None
+  end.
+
 Fixpoint regcol_extract (r : reg_kind) (regs : list (reg_kind * valu_shape)) : option (valu_shape * list (reg_kind * valu_shape)) :=
   match regs with
   | (r', s)::regs' =>
@@ -1247,19 +1263,8 @@ Section instances.
      (find_in_context (FindStructRegMapsTo r f) (λ rk,
       match rk with
       | RKMapsTo v' => (⌜vread = v'⌝ -∗ r # f ↦ᵣ v' -∗ WPasm es)
-      | RKCol regs => tactic_hint (vm_compute_hint (list_find_idx_bool (λ x,
-            reg_kind_eqb x.1 (KindField r f) || (reg_kind_eqb x.1 (KindReg r) &&
-                   let r := (match x.2 with
-              | ExactShape (RegVal_Struct rs) => list_find_idx_bool (λ y, String.eqb y.1 f) rs
-              | StructShape ss => list_find_idx (λ y, String.eqb y.1 f) ss
-              | _ => None
-              end) in
-              match r with
-              | Some _ => true
-              | _ => false
-              end))) regs) (λ i,
-               ⌜if (regs !!! i).1 is KindField _ _ then valu_has_shape vread (regs !!! i).2 else True⌝ -∗
-               (reg_col regs -∗ WPasm es))
+      | RKCol regs => tactic_hint (regcol_compute_hint (regcol_lookup_field r f) regs) (λ '(b, s),
+             ⌜if b then valu_has_shape vread s else True⌝ -∗ reg_col regs -∗ WPasm es)
       end))) -∗
     WPasm (ReadReg r [Field f] v ann :t: es).
   Proof. Admitted.
@@ -1320,22 +1325,18 @@ Section instances.
     ((find_in_context (FindStructRegMapsTo r f) (λ rk,
       match rk with
       | RKMapsTo v' => ⌜v = v'⌝ ∗ (r # f ↦ᵣ v' -∗ WPasm es)
-      | RKCol regs => tactic_hint (vm_compute_hint (list_find_idx (λ x, x.1 = KindField r f ∨ x.1 = KindReg r)%type) regs) (λ i,
-          ∃ e, ⌜e = (regs !!! i)⌝ ∗
-          match e.1 with
-          | KindField _ _ => ⌜e.2 = ExactShape v⌝ ∗ (reg_col regs -∗ WPasm es)
-          | KindReg _ =>
-              if e.2 is ExactShape (RegVal_Struct rs) then
-                tactic_hint (vm_compute_hint (list_find_idx (λ x, x.1 = f)) rs) (λ i,
-                  ⌜(rs !!! i).2 = v⌝ ∗ (reg_col regs -∗ WPasm es)) else False
-          end)
+      | RKCol regs => tactic_hint (regcol_compute_hint (regcol_lookup_field r f) regs) (λ '(b, s),
+          if s is ExactShape v' then ⌜v = v'⌝ ∗ (reg_col regs -∗ WPasm es) else False)
       end))) -∗
     WPasm (AssumeReg r [Field f] v ann :t: es).
   Proof.
     unfold tactic_hint, vm_compute_hint.
     iDestruct 1 as (?) "[Hr Hwp]" => /=. case_match; simplify_eq.
     - iDestruct "Hwp" as (->) "?". by iApply (wp_assume_reg_struct with "Hr").
-    - iDestruct "Hwp" as (i [[??][?[Hor ?]]]%list_find_idx_Some) "Hwp"; simplify_eq/=.
+    -
+  Admitted.
+  (*
+      iDestruct "Hwp" as (i [[??][?[Hor ?]]]%list_find_idx_Some) "Hwp"; simplify_eq/=.
       erewrite list_lookup_total_correct; [|done].
       iDestruct "Hwp" as (e ->) "Hwp"; simplify_eq/=. destruct Hor; simplify_eq.
       + iDestruct "Hwp" as (->) "Hwp".
@@ -1352,7 +1353,7 @@ Section instances.
         iIntros "Hr". iApply "Hwp". iApply "Hregs".
         iExists _. by iFrame.
   Qed.
-
+*)
   Lemma li_wp_write_reg r v ann es:
     (find_in_context (FindRegMapsTo r) (λ rk,
       match rk with
@@ -1548,24 +1549,18 @@ Section instances.
     (find_in_context (FindStructRegMapsTo r f) (λ rk,
       match rk with
       | RKMapsTo v => (if v is RegVal_Base v' then r # f ↦ᵣ v -∗ Φ v' else False)
-      | RKCol regs => tactic_hint (vm_compute_hint (list_find_idx (λ x, x.1 = KindField r f ∨ x.1 = KindReg r)%type) regs) (λ i,
-          ∃ e, ⌜e = (regs !!! i)⌝ ∗
-          match e.1 with
-          | KindField _ _ =>
-              ∀ v, ⌜valu_has_shape v e.2⌝ -∗ ∃ v', ⌜v = RegVal_Base v'⌝ ∗ (reg_col regs -∗ Φ v')
-          | KindReg _ =>
-              ∀ v, ⌜valu_has_shape v e.2⌝ -∗ ∃ rs, ⌜v = RegVal_Struct rs⌝ ∗
-                tactic_hint (vm_compute_hint (list_find_idx (λ x, x.1 = f)) rs) (λ i,
-                  if (rs !!! i).2 is RegVal_Base v' then reg_col regs -∗ Φ v' else False
-                 )
-          end)
+      | RKCol regs => tactic_hint (regcol_compute_hint (regcol_lookup_field r f) regs) (λ '(b, s),
+           ∀ v, ⌜valu_has_shape v s⌝ -∗ if v is RegVal_Base v' then (reg_col regs -∗ Φ v') else False)
       end)) -∗
     WPaexp (AExp_Val (AVal_Var r [Field f]) ann) {{ Φ }}.
   Proof.
     unfold tactic_hint, vm_compute_hint.
     iDestruct 1 as (rk) "[Hr Hwp]" => /=. case_match; simplify_eq.
     - case_match => //; subst. by iApply (wpae_var_struct with "Hr").
-    - iDestruct "Hwp" as (? [[??][?[Hor ?]]]%list_find_idx_Some) "Hwp"; simplify_eq/=.
+    -
+  Admitted.
+  (*
+      iDestruct "Hwp" as (? [[??][?[Hor ?]]]%list_find_idx_Some) "Hwp"; simplify_eq/=.
       erewrite list_lookup_total_correct; [|done].
       iDestruct "Hwp" as (e ->) "Hwp"; simplify_eq/=. destruct Hor; simplify_eq.
       + iDestruct (big_sepL_lookup_acc with "Hr") as "[[%vact [% Hr]] Hregs]"; [done|]; simplify_eq/=.
@@ -1580,7 +1575,7 @@ Section instances.
         { rewrite /read_accessor /=. by simplify_option_eq. }
         iIntros "Hr". iApply "Hwp". iApply "Hregs". iExists _. by iFrame.
   Qed.
-
+*)
   Lemma li_wpae_bits b Φ ann:
     Φ (Val_Bits b) -∗
     WPaexp (AExp_Val (AVal_Bits b) ann) {{ Φ }}.
